src/Enumeration/Loopers.dfy
@@ -1,21 +1,22 @@
 
-include "../Actions.dfy"
+// include "../Actions.dfy"
 include "../Frames.dfy"
+include "../Wrappers.dfy"
 
 module Loopers {
 
-  import opened Actions
+  // import opened Actions
   import opened Frames
+  import opened Wrappers
 
-  trait Looper {
-    predicate Invariant()
+  trait InfiniteStepper extends Validatable {
     method Step() 
-      requires Invariant()
-      ensures Invariant()
+      requires Valid()
+      ensures Valid()
   }
 
-  method DoLoopStar(l: Looper) 
-    requires l.Invariant()
+  method DoLoopStar(l: InfiniteStepper) 
+    requires l.Valid()
     decreases *
   {
     while (true) decreases * {
@@ -23,18 +24,7 @@ module Loopers {
     }
   }
 
-  trait TerminatingLooper extends Validatable {
-    // Would be better as an arbitrary termination clause somehow instead
-    // https://github.com/dafny-lang/dafny/issues/762
-    function Decreases(): nat
-      reads Repr
-      decreases Repr
-      requires Valid()
-    predicate method Done() 
-      reads Repr
-      requires Valid()
-      ensures Decreases() == 0 ==> Done()
-
+  trait Stepper extends Validatable {
     method Step() 
       requires Valid()
       requires !Done()
@@ -42,25 +32,63 @@ module Loopers {
       decreases Repr
       ensures ValidAndDisjoint()
       ensures Decreases() < old(Decreases())
+
+    // Would be better as an arbitrary termination clause somehow instead
+    // https://github.com/dafny-lang/dafny/issues/762
+    function Decreases(): nat
+      reads Repr
+      decreases Repr
+      requires Valid()
+
+    predicate method Done() 
+      reads Repr
+      requires Valid()
+      decreases Repr, 0
+      ensures Decreases() == 0 ==> Done()
   }
 
-  method DoLoop(l: TerminatingLooper) 
+  method DoLoop(l: Stepper)
     requires l.Valid()
     modifies l.Repr
     ensures l.Valid()
     ensures l.Done()
   {
     while (!l.Done())
-      invariant l.Valid()
-      // Could this be a more general Ensures or Invariant?
-      invariant fresh(l.Repr - old(l.Repr))
+      invariant l.ValidAndDisjoint()
       decreases l.Decreases()
     {
       l.Step();
     }
   }
 
-  class SeqLooper<T> extends TerminatingLooper {
+  trait Enumerator<T> extends Stepper {
+
+    // Any enumerator that produces one value at a time
+    // and provably terminates is equivalent to an enumerator
+    // that produces a specific seq<T>. This value may be underspecified
+    // such that it is not known, even its length, until after all
+    // values have been produced.
+    // Dafny doesn't let you pass around an underspecified value though,
+    // so we don't define a "to be enumerated" field or function.
+    
+    ghost var enumerated: seq<T>
+
+    method Step()
+      requires Valid()
+      requires !Done()
+      modifies Repr
+      decreases Repr
+      ensures ValidAndDisjoint()
+      ensures Decreases() < old(Decreases())
+      ensures enumerated == old(enumerated) + [old(Current())]
+
+    function method Current(): T
+      reads this, Repr
+      requires Valid()
+      requires !Done()
+  }
+
+  class SeqEnumerator<T> extends Enumerator<T> {
 
     const elements: seq<T>
     var index: nat
@@ -71,6 +99,8 @@ module Loopers {
     {
       elements := s;
       index := 0;
+
+      enumerated := [];
       Repr := {this};
     }
 
@@ -81,6 +111,7 @@ module Loopers {
     {
       && this in Repr
       && 0 <= index <= |elements|
+      && enumerated == elements[0..index]
     }
 
     function Decreases(): nat
@@ -93,7 +124,9 @@ module Loopers {
     predicate method Done() 
       reads Repr
       requires Valid()
+      decreases Repr, 0
       ensures Decreases() == 0 ==> Done()
+      ensures Done() ==> enumerated == elements
     {
       index == |elements|
     }
@@ -105,9 +138,117 @@ module Loopers {
       decreases Repr
       ensures ValidAndDisjoint()
       ensures Decreases() < old(Decreases())
+      ensures enumerated == old(enumerated) + [old(Current())]
     {
+      enumerated := enumerated + [Current()];
       index := index + 1;
     }
+
+    function method Current(): T
+      reads this, Repr
+      requires Valid()
+      requires !Done()
+    {
+      elements[index]
+    }
+  }
+
+  // Wraps an enumerator that doesn't know if it has another value
+  // until it tries to get the next value.
+  // TODO: Equivalent to Filter?
+  class TerminatedEnumerator<T> extends Enumerator<T> {
+    const wrapped: Enumerator<Option<T>>
+
+    constructor(wrapped: Enumerator<Option<T>>) 
+      requires wrapped.Valid()
+      ensures Valid()
+      ensures fresh(Repr - {this} - wrapped.Repr)
+    {
+      this.wrapped := wrapped;
+      enumerated := [];
+      Repr := {this} + wrapped.Repr;
+    }
+
+    predicate Valid() 
+      reads this, Repr 
+      ensures Valid() ==> this in Repr 
+      decreases Repr
+    {
+      && this in Repr
+      && ValidComponent(wrapped)
+    }
+
+    function Decreases(): nat
+      reads Repr
+      requires Valid()
+    {
+      wrapped.Decreases()
+    }
+
+    predicate method Done() 
+      reads Repr
+      requires Valid()
+      decreases Repr, 0
+      ensures Decreases() == 0 ==> Done()
+    {
+      wrapped.Done() || wrapped.Current().None?
+    }
+
+    method Step()
+      requires Valid()
+      requires !Done()
+      modifies Repr
+      decreases Repr
+      ensures ValidAndDisjoint()
+      ensures Decreases() < old(Decreases())
+      ensures enumerated == old(enumerated) + [old(Current())]
+    {
+      enumerated := enumerated + [Current()];
+      wrapped.Step();
+      Repr := {this} + wrapped.Repr;
+    }
+
+    function method Current(): T
+      reads this, Repr
+      requires Valid()
+      requires !Done()
+    {
+      wrapped.Current().value
+    }
+  }
+
+  method Example1() {
+    var numbers := [1, 2, 3, 4, 5];
+    var e: Enumerator<int> := new SeqEnumerator(numbers);
+    label start:
+    while (!e.Done()) 
+      invariant e.Valid()
+      invariant old@start(allocated(e)) && fresh(e.Repr)
+      decreases e.Decreases()
+    {
+      print e.Current(), "\n";
+      e.Step();
+    }
+  }
+
+  method Example2() {
+    var maybeNumbers := [Some(1), Some(2), Some(3), None, None];
+    var e: Enumerator<Option<int>> := new SeqEnumerator(maybeNumbers);
+    var e': Enumerator<int> := new TerminatedEnumerator(e);
+    label start:
+    while (!e'.Done()) 
+      invariant e'.Valid()
+      invariant old@start(allocated(e')) && fresh(e'.Repr)
+      decreases e'.Decreases()
+    {
+      print e'.Current(), "\n";
+      e'.Step();
+    }
+  }
+
+  method Main() {
+    Example1();
+    Example2();
   }
 
   // TODO: Some similarities between this and composing
@@ -122,134 +263,134 @@ module Loopers {
   //   var _ := action.Invoke(r2);
   //   ...
   
-  class ForEach extends TerminatingLooper {
-    const iter: TerminatingLooper
-    const body: Action<TerminatingLooper, ()>
+  // class ForEach extends TerminatingLooper {
+  //   const iter: TerminatingLooper
+  //   const body: Action<TerminatingLooper, ()>
 
-    constructor(iter: TerminatingLooper, body: Action<TerminatingLooper, ()>)
-      requires iter.Valid()
-      requires body.Valid()
-      requires iter.Repr !! body.Repr
-      requires iter.Valid() ==> body.Requires(iter)
-      requires iter.Valid() ==> body.Modifies(iter) !! iter.Repr
-      ensures Valid()
-    {
-      this.iter := iter;
-      this.body := body;
-      Repr := {this} + iter.Repr + body.Repr;
-    }
+  //   constructor(iter: TerminatingLooper, body: Action<TerminatingLooper, ()>)
+  //     requires iter.Valid()
+  //     requires body.Valid()
+  //     requires iter.Repr !! body.Repr
+  //     requires iter.Valid() ==> body.Requires(iter)
+  //     requires iter.Valid() ==> body.Modifies(iter) !! iter.Repr
+  //     ensures Valid()
+  //   {
+  //     this.iter := iter;
+  //     this.body := body;
+  //     Repr := {this} + iter.Repr + body.Repr;
+  //   }
 
-    predicate Valid() 
-      reads this, Repr
-      decreases Repr
-      ensures Valid() ==> this in Repr
-    {
-      && this in Repr
-      && ValidComponent(iter)
-      && ValidComponent(body)
-      && iter.Repr !! body.Repr
-      && (iter.Valid() ==> body.Requires(iter))
-      // TODO: This needs to be a forall somehow
-      && (iter.Valid() ==> body.Modifies(iter) !! iter.Repr)
-    }
+  //   predicate Valid() 
+  //     reads this, Repr
+  //     decreases Repr
+  //     ensures Valid() ==> this in Repr
+  //   {
+  //     && this in Repr
+  //     && ValidComponent(iter)
+  //     && ValidComponent(body)
+  //     && iter.Repr !! body.Repr
+  //     && (iter.Valid() ==> body.Requires(iter))
+  //     // TODO: This needs to be a forall somehow
+  //     && (iter.Valid() ==> body.Modifies(iter) !! iter.Repr)
+  //   }
 
-    function Decreases(): nat 
-      reads Repr
-      requires Valid()
-    {
-      iter.Decreases()
-    }
+  //   function Decreases(): nat 
+  //     reads Repr
+  //     requires Valid()
+  //   {
+  //     iter.Decreases()
+  //   }
 
-    predicate method Done() 
-      reads Repr
-      requires Valid()
-      ensures Decreases() == 0 ==> Done()
-    {
-      iter.Done()
-    }
+  //   predicate method Done() 
+  //     reads Repr
+  //     requires Valid()
+  //     ensures Decreases() == 0 ==> Done()
+  //   {
+  //     iter.Done()
+  //   }
 
-    method Step() 
-      requires Valid()
-      requires !Done()
-      modifies Repr
-      decreases Repr
-      ensures ValidAndDisjoint()
-      ensures Decreases() < old(Decreases())
-    {
-      iter.Step();
-      Repr := Repr + iter.Repr;
+  //   method Step() 
+  //     requires Valid()
+  //     requires !Done()
+  //     modifies Repr
+  //     decreases Repr
+  //     ensures ValidAndDisjoint()
+  //     ensures Decreases() < old(Decreases())
+  //   {
+  //     iter.Step();
+  //     Repr := Repr + iter.Repr;
 
-      assert iter.Valid();
-      assert  this in Repr;
-      assert  ValidComponent(iter);
-      assert  ValidComponent(body);
-      assert  iter.Repr !! body.Repr;
-      assert  (iter.Valid() ==> body.Requires(iter));
-      assert  (iter.Valid() ==> body.Modifies(iter) !! iter.Repr);
-      assert Valid();
+  //     assert iter.Valid();
+  //     assert  this in Repr;
+  //     assert  ValidComponent(iter);
+  //     assert  ValidComponent(body);
+  //     assert  iter.Repr !! body.Repr;
+  //     assert  (iter.Valid() ==> body.Requires(iter));
+  //     assert  (iter.Valid() ==> body.Modifies(iter) !! iter.Repr);
+  //     assert Valid();
       
-      var _ := body.Invoke(iter);
-      Repr := Repr + body.Repr;
-    }
-  }
+  //     var _ := body.Invoke(iter);
+  //     Repr := Repr + body.Repr;
+  //   }
+  // }
 
-  class SeqCollector<T> extends Action<T, ()> {
+  // class SeqCollector<T> extends Action<T, ()> {
 
-    var elements: seq<T>
+  //   var elements: seq<T>
 
-    constructor() 
-      ensures Valid()
-      ensures fresh(Repr - {this})
-    {
-      elements := [];
-      Repr := {this};
-    }
+  //   constructor() 
+  //     ensures Valid()
+  //     ensures fresh(Repr - {this})
+  //   {
+  //     elements := [];
+  //     Repr := {this};
+  //   }
 
-    predicate Valid() 
-      reads this, Repr 
-      ensures Valid() ==> this in Repr 
-      decreases Repr
-    {
-      && this in Repr
-    }
+  //   predicate Valid() 
+  //     reads this, Repr 
+  //     ensures Valid() ==> this in Repr 
+  //     decreases Repr
+  //   {
+  //     && this in Repr
+  //   }
 
-    method Invoke(t: T) returns (nothing: ())
-      requires Valid()
-      requires Requires(t)
-      modifies Modifies(t)
-      decreases Decreases(t)
-      ensures ValidAndDisjoint()
-      ensures old(allocated(())) && Ensures(t, ())
-    {
-      elements := elements + [t];
-    }
+  //   method Invoke(t: T) returns (nothing: ())
+  //     requires Valid()
+  //     requires Requires(t)
+  //     modifies Modifies(t)
+  //     decreases Decreases(t)
+  //     ensures ValidAndDisjoint()
+  //     ensures old(allocated(())) && Ensures(t, ())
+  //   {
+  //     elements := elements + [t];
+  //   }
 
-    predicate Requires(t: T) {
-      true
-    }
+  //   predicate Requires(t: T) {
+  //     true
+  //   }
 
-    // Need this separately from Repr for callers
-    // Repr is the frame for Valid(), but callers
-    // need to know what ELSE gets modified.
-    function Modifies(t: T): set<object> requires Requires(t) {
-      {this}
-    }
+  //   // Need this separately from Repr for callers
+  //   // Repr is the frame for Valid(), but callers
+  //   // need to know what ELSE gets modified.
+  //   function Modifies(t: T): set<object> requires Requires(t) {
+  //     {this}
+  //   }
 
-    function Decreases(t: T): nat {
-      0
-    }
+  //   function Decreases(t: T): nat {
+  //     0
+  //   }
     
-    twostate predicate Ensures(t: T, nothing: ()) {
-      true
-    }
-  }
+  //   twostate predicate Ensures(t: T, nothing: ()) {
+  //     true
+  //   }
+  // }
 
 
-  method Main() {
-    var numbers := [1, 2, 3, 4, 5];
-    var numbersIter := new SeqLooper(numbers);
-    var numbersPrinterLooper := new SeqCollector();
-    var forEachLoop := new ForEach(numbersIter, numbersPrinterLooper);
-    DoLoop(forEachLoop);
-  }
+  // method Main() {
+  //   var numbers := [1, 2, 3, 4, 5];
+  //   var numbersIter := new SeqLooper(numbers);
+  //   var numbersPrinterLooper := new SeqCollector();
+  //   var forEachLoop := new ForEach(numbersIter, numbersPrinterLooper);
+  //   DoLoop(forEachLoop);
+  // }
 }
